writing new fixpoint

theories/ub_logic/ub_weakestpre.v
@@ -223,7 +223,7 @@ Section exec_ub.
   Proof.
     iApply exec_ub_strong_mono; [iPureIntro; lra | ].
     iIntros (???) "[[% ?] ?]". iSplit; [|done]. by iExists _.
-xo  Qed.
+  Qed.
 
   Lemma exec_ub_bind K `{!LanguageCtx K} e1 σ1 (Z : nonnegreal -> cfg Λ → iProp Σ) (ε : nonnegreal) :
     to_val e1 = None →
@@ -544,6 +544,196 @@ xo  Qed.
   *)
 
 End exec_ub.
+
+
+Section exec_ub_limit.
+  Context `{!irisGS Λ Σ}.
+
+  Definition exec_ub_limit_pre (Z : nonnegreal -> cfg Λ → iProp Σ) (Φ : nonnegreal * cfg Λ → iProp Σ) :=
+    (λ (x : nonnegreal * cfg Λ),
+       let '(ε, (e1, σ1)) := x in
+       (* [prim_step] *)
+       (∃ R (ε1 ε2 : nat -> nonnegreal), ⌜ (Inf_seq ε1 + Inf_seq ε2 <= ε)%R ⌝ ∗ ⌜∀ n, ub_lift (prim_step e1 σ1) R (ε1 n)⌝ ∗ ∀ ρ2 n, ⌜ R ρ2 ⌝ ={∅}=∗ Z (ε2 n) ρ2 ) ∨
+         (* [prim_step] with adv composition *)
+         (∃ R (ε1 : nat -> nonnegreal) (ε2 : cfg Λ -> nat -> nonnegreal),
+             ⌜ exists r, forall ρ, (Inf_seq (ε2 ρ) <= r)%R ⌝ ∗ ⌜ (Inf_seq ε1 + SeriesC (λ ρ, (prim_step e1 σ1 ρ) * Inf_seq (ε2 ρ)) <= ε)%R ⌝ ∗ ⌜∀ n, ub_lift (prim_step e1 σ1) R (ε1 n)⌝ ∗
+                                                                                                                                         ∀ ρ2 n, ⌜ R ρ2 ⌝ ={∅}=∗ Z (ε2 ρ2 n) ρ2 ) ∨
+         (* [state_step]  *)
+         ([∨ list] α ∈ get_active σ1,
+            (* We allow an explicit weakening of the grading, but maybe it is not needed *)
+            (∃ R (ε1 ε2 : nat -> nonnegreal), ⌜ (Inf_seq ε1 + Inf_seq ε2 <= ε)%R ⌝ ∗ ⌜∀ n, ub_lift (state_step σ1 α) R (ε1 n) ⌝ ∗ ∀ σ2 n, ⌜ R σ2 ⌝ ={∅}=∗ Φ (ε2 n,((e1, σ2)))))
+    )%I.
+
+  Local Instance exec_state_ub_limit_pre_NonExpansive Z Φ :
+    NonExpansive (exec_ub_limit_pre Z Φ).
+  Proof.
+    rewrite /exec_ub_limit_pre.
+    intros n [?[??]] [?[??]] [[=][[=][=]]].
+    by subst.
+  Qed.
+
+  Local Instance exec_coupl_limit_pre_mono Z : BiMonoPred (exec_ub_limit_pre Z).
+  Proof.
+    split; last apply _.
+    iIntros (Φ Ψ HNEΦ HNEΨ) "#Hwand".
+    rewrite /exec_ub_limit_pre.
+    iIntros ([ε[e σ]]) "Hexec".
+    iDestruct "Hexec" as "[H|[H|H]]".
+    - by iLeft.
+    - by iRight; iLeft.
+    - iRight. iRight.
+      iInduction (get_active σ) as [|l] "IH" forall "H".
+      { rewrite big_orL_nil //. }
+      rewrite !big_orL_cons.
+      iDestruct "H" as "[H|H]".
+      + iLeft. 
+        iDestruct "H" as "[%R H]".
+        iExists R.
+        iDestruct "H" as "(%&%&%&%&H)".
+        iExists _, _. iSplitR; [done|].
+        iSplitR; [done|].
+        iIntros. iApply "Hwand". by iApply "H".
+      + iRight. by iApply "IH".
+  Qed.
+
+  
+  Definition exec_ub_limit' Z := bi_least_fixpoint (exec_ub_limit_pre Z).
+  Definition exec_ub_limit e σ Z ε := exec_ub_limit' Z (ε, (e, σ)).
+
+  Lemma exec_ub_limit_unfold e1 σ1 Z ε :
+    exec_ub_limit e1 σ1 Z ε ≡
+      ((* [prim_step] *)
+        (∃ R (ε1 ε2 : nat -> nonnegreal), ⌜ (Inf_seq ε1 + Inf_seq ε2 <= ε)%R ⌝ ∗ ⌜∀ n, ub_lift (prim_step e1 σ1) R (ε1 n)⌝ ∗ ∀ ρ2 n, ⌜ R ρ2 ⌝ ={∅}=∗ Z (ε2 n) ρ2 ) ∨
+          (* [prim_step] with adv composition *)
+          (∃ R (ε1 : nat -> nonnegreal) (ε2 : cfg Λ -> nat -> nonnegreal),
+              ⌜ exists r, forall ρ, (Inf_seq (ε2 ρ) <= r)%R ⌝ ∗
+                          ⌜ (Inf_seq ε1 + SeriesC (λ ρ, (prim_step e1 σ1 ρ) * Inf_seq (ε2 ρ)) <= ε)%R ⌝ ∗ ⌜∀ n, ub_lift (prim_step e1 σ1) R (ε1 n)⌝ ∗ ∀ ρ2 n, ⌜ R ρ2 ⌝ ={∅}=∗ Z (ε2 ρ2 n) ρ2 ) ∨
+          (* [state_step]  *)
+          ([∨ list] α ∈ get_active σ1,
+             (* We allow an explicit weakening of the grading, but maybe it is not needed *)
+             (∃ R (ε1 ε2 : nat -> nonnegreal), ⌜ (Inf_seq ε1 + Inf_seq ε2 <= ε)%R ⌝ ∗ ⌜∀ n, ub_lift (state_step σ1 α) R (ε1 n) ⌝ ∗ ∀ σ2 n, ⌜ R σ2 ⌝ ={∅}=∗ exec_ub_limit e1 σ2 Z (ε2 n)  )))%I.
+  Proof.  rewrite /exec_ub_limit/exec_ub_limit' least_fixpoint_unfold //. Qed.
+
+  
+  Local Lemma inf_seq_nonnegreal_nonneg (f:nat -> nonnegreal): 0<=Inf_seq f.
+  Proof.
+    rewrite Inf_opp_sup Rbar_opp_real.
+    apply Ropp_0_ge_le_contravar.
+    apply Rle_ge.
+    replace 0 with (real (Finite 0)); last done.
+    apply finite_rbar_le.
+    + eapply (is_finite_bounded (- (f 0%nat)) 0).
+      -- eapply (Sup_seq_minor_le _ _ 0%nat).
+         rewrite /nonneg. simpl. destruct (f 0%nat). done.
+      -- apply upper_bound_ge_sup. intros. rewrite /nonneg.
+         destruct (f n) as [x Hx].
+         apply Ropp_le_contravar in Hx.
+         replace (-0) with 0 in Hx; try done.
+         lra.
+    + apply upper_bound_ge_sup. intros. rewrite /nonneg.
+      destruct (f n) as [x Hx].
+      apply Ropp_le_contravar in Hx.
+      replace (-0) with 0 in Hx; try done.
+      lra.
+  Qed.
+
+  Local Lemma inf_seq_exists_index (f:nat -> nonnegreal) ε:
+    Inf_seq (λ x : nat, f x) < ε -> ∃ n : nat, f n <= ε.
+  Proof.
+    Admitted.
+  
+  Lemma exec_ub_limit_implies_exec_ub e σ Z ε :
+    exec_ub_limit e σ Z ε -∗ exec_ub e σ Z ε.
+  Proof.
+    rewrite /exec_ub_limit/exec_ub_limit'/exec_ub/exec_ub'.
+    iIntros "Hlimit".
+    iApply (least_fixpoint_strong_mono with "[][$Hlimit]").
+    { apply exec_coupl_pre_mono. }
+    iModIntro.
+    clear e σ ε.
+    iIntros (Φ [ε [e1 σ1]]).
+    rewrite /exec_ub_limit_pre/exec_ub_pre.
+    iIntros "[H|[H|H]]".
+    - iLeft. iDestruct "H" as "[%R H]".
+      iExists R. iDestruct "H" as "(%ε1 & %ε2 & %Hε & %Hstep &H)".
+      iExists (mknonnegreal (real (Inf_seq ε1)) _), (mknonnegreal (real (Inf_seq ε2)) _).
+      simpl. iSplitR.
+      { done. }
+      iSplitR.
+      { iPureIntro.
+        apply ub_lift_epsilon_limit.
+        + apply Rle_ge. apply inf_seq_nonnegreal_nonneg.
+        + intros.
+          assert (∃ n, ε1 n <= ε0) as [n Hn].
+          { apply inf_seq_exists_index. lra.  }
+          eapply UB_mon_grading; [apply Hn|done].
+      }
+      iIntros ([??]) "%R'". 
+      admit.
+    - iRight; iLeft. iDestruct "H" as "[%R H]".
+      iExists R. admit.
+    - iRight; iRight. admit. 
+  Admitted.
+
+  Lemma exec_ub_implies_exec_ub_limit e σ Z ε :
+    exec_ub e σ Z ε -∗ exec_ub_limit e σ Z ε.
+  Proof.
+    rewrite /exec_ub/exec_ub'/exec_ub_limit/exec_ub_limit'.
+    iIntros "Hlimit".
+    iApply (least_fixpoint_strong_mono with "[][$Hlimit]").
+    { apply exec_coupl_pre_mono. }
+    iModIntro.
+    clear e σ ε.
+    iIntros (Φ [ε [e1 σ1]]).
+    rewrite /exec_ub_limit_pre/exec_ub_pre.
+    iIntros "[H|[H|H]]".
+    - iLeft. iDestruct "H" as "(%R & %ε1 & %ε2 & %Hε & %Hub & H)".
+      iExists R, (λ _, ε1), (λ _, ε2).
+      iSplitR.
+      { iPureIntro; rewrite !Inf_opp_sup !Rbar_opp_real !sup_seq_const.
+        lra.
+      }
+      iSplitR.
+      { iPureIntro; by intros. }
+      iIntros. by iApply "H".
+    - iRight; iLeft. iDestruct "H" as "(%R & %ε1 & %ε2 & %Hbound & %Hε & %Hub & H)".
+      iExists R, (λ _, ε1), (λ s _, ε2 s).
+      iSplitR.
+      { iPureIntro. destruct Hbound as [r Hbound]. exists r.
+        intros. rewrite !Inf_opp_sup !Rbar_opp_real !sup_seq_const.
+        replace (--_) with (nonneg (ε2 ρ)) by lra.
+        eauto.
+      }
+      iSplitR.
+      { iPureIntro. erewrite SeriesC_ext; last first.
+        - intros. rewrite !Inf_opp_sup !Rbar_opp_real !sup_seq_const.
+          replace (--_) with (nonneg (ε2 n)) by lra.
+          done.
+        - rewrite !Inf_opp_sup !Rbar_opp_real !sup_seq_const.
+          lra.
+      }
+      iSplitR.
+      { iPureIntro; eauto. }
+      iIntros; by iApply "H".
+    - iRight; iRight.
+      iInduction (get_active σ1) as [|l] "IH".
+      { by rewrite big_orL_nil //. }
+      rewrite 2!big_orL_cons. iDestruct "H" as "[H|H]".
+      + iLeft. iDestruct "H" as "(%R & %ε1 & %ε2 & %Hε & %Hstate & H)".
+        iExists R, (λ _, ε1), (λ _, ε2).
+        iSplitR.
+        { iPureIntro. rewrite !Inf_opp_sup !Rbar_opp_real !sup_seq_const.
+          lra.
+        }
+        iSplitR.
+        { iPureIntro. by intros. }
+        iIntros. by iApply "H".
+      + iRight. by iApply "IH".
+  Qed. 
+    
+End exec_ub_limit.
+          
+
 
 (** * The weakest precondition  *)
 Definition ub_wp_pre `{!irisGS Λ Σ}
