theories/ub_logic/adequacy.v
@@ -228,100 +228,6 @@ Proof.
 Qed.
 
 
-(*epsilon limit*)
-Lemma ub_lift_epsilon_limit `{Eq: EqDecision A} `{HC:Countable A} (μ : distr A) f ε':
-  ε'>=0 -> (forall ε, ε>ε' -> ub_lift μ f ε) -> ub_lift μ f ε'.
-Proof.
-  intros Hε' H.
-  assert (forall seq,(∃ b, ∀ n, 0 <= - seq n <= b) -> (∀ n, ub_lift μ f (ε'-seq n))->ub_lift μ f (ε'-Sup_seq seq)) as H_limit.
-  { clear H.
-    rewrite /ub_lift.
-    intros.
-    rewrite Rcomplements.Rle_minus_r.
-    rewrite Rplus_comm.
-    rewrite -Rcomplements.Rle_minus_r.
-    rewrite <- rbar_le_rle.
-    rewrite rbar_finite_real_eq.
-    + apply upper_bound_ge_sup.
-      intros.
-      pose proof (H0 n P H1). rewrite rbar_le_rle. lra.
-    + destruct H as [b H].
-      apply (is_finite_bounded (-b) 0).
-      -- eapply (Sup_seq_minor_le _ _ 0). destruct (H 0%nat). apply Ropp_le_contravar in H3.
-         rewrite Ropp_involutive in H3. apply H3.
-      -- apply upper_bound_ge_sup. intros n. destruct (H n). apply Ropp_le_contravar in H2.
-         rewrite Ropp_involutive in H2. rewrite Ropp_0 in H2. done.
-  }
-  replace ε' with (ε'- Sup_seq (λ x,(λ n,-1%R/(S n)) x)).
-  - apply H_limit.
-    { exists 1.
-      intros; split.
-      -- rewrite Ropp_div. rewrite Ropp_involutive.
-         apply Rcomplements.Rdiv_le_0_compat; try lra.
-         rewrite S_INR. pose proof (pos_INR n).
-         lra.
-      -- rewrite Ropp_div. rewrite Ropp_involutive.
-         rewrite Rcomplements.Rle_div_l; [|apply Rlt_gt].
-         ++ assert (1<=S n); try lra.
-            rewrite S_INR.
-            pose proof (pos_INR n).
-            lra.
-         ++ rewrite S_INR.
-            pose proof (pos_INR n).
-            lra. 
-    }
-    intros. apply H.
-    assert (1/(S n) > 0); try lra.
-    apply Rlt_gt.
-    apply Rdiv_lt_0_compat; first lra.
-    rewrite S_INR. pose proof (pos_INR n); lra.
-  - assert (Sup_seq (λ x : nat, - (1)%R / S x)=0) as Hswap; last first.
-    + rewrite Hswap. erewrite<- eq_rbar_finite; [|done]. lra.
-    + apply is_sup_seq_unique. rewrite /is_sup_seq.
-      intros err.
-      split.
-      -- intros n.
-         eapply (Rbar_le_lt_trans _ (Rbar.Finite 0)); last first.
-         ++ rewrite Rplus_0_l. apply (cond_pos err).  
-         ++ apply Rge_le. rewrite Ropp_div. apply Ropp_0_le_ge_contravar.
-            apply Rcomplements.Rdiv_le_0_compat; try lra.
-            rewrite S_INR. pose proof (pos_INR n); lra.
-      -- pose (r := 1/err -1).
-         assert (exists n, r<INR n) as [n Hr]; last first.
-         ++ eexists n.
-            erewrite Ropp_div. replace (_-_) with (- (pos err)) by lra.
-            apply Ropp_lt_contravar.
-            rewrite Rcomplements.Rlt_div_l.
-            2:{ rewrite S_INR. pose proof pos_INR. apply Rlt_gt.
-                eapply Rle_lt_trans; [eapply H0|].
-                apply Rlt_n_Sn.
-            }
-            rewrite S_INR.
-            rewrite Rmult_comm.
-            rewrite <-Rcomplements.Rlt_div_l.
-            2:{ pose proof (cond_pos err); lra. }
-            rewrite <- Rcomplements.Rlt_minus_l.
-            rewrite -/r. done.
-         ++ pose proof (Rgt_or_ge 0 r).
-            destruct H0.
-            --- exists 0%nat. eapply Rlt_le_trans; last apply pos_INR.
-                lra.
-            --- exists (Z.to_nat (up r)).
-                pose proof (archimed r) as [? ?].
-                rewrite INR_IZR_INZ.
-                rewrite ZifyInst.of_nat_to_nat_eq.
-                rewrite /Z.max.
-                case_match.
-                { rewrite Z.compare_eq_iff in H3.
-                  exfalso. rewrite -H3 in H1. lra.
-                }
-                2: { rewrite Z.compare_gt_iff in H3. exfalso.
-                     assert (IZR (up r) >= 0) by lra.
-                     apply IZR_lt in H3. lra. 
-                }
-                lra.
-Qed.
-
 
 Lemma exec_ub_epsilon_limit `{ub_clutchGS Σ} (e : expr) σ Z (ε':nonnegreal):
    (∀ ε : nonnegreal, ⌜ε > ε'⌝ -∗ exec_ub e σ Z ε) -∗ exec_ub e σ Z ε'.
@@ -388,7 +294,10 @@ Section Experiment_exec_ub_no_chain.
     destruct c as [e σ].
     Abort.
     
-End Experiment_exec_ub_no_chain.y
+End Experiment_exec_ub_no_chain.
+
+
+
 
 Lemma wp_epsilon_limit `{ub_clutchGS Σ} (e : expr) φ:
    (∀ ε : nonnegreal, ⌜0<ε⌝ -∗ € ε -∗ WP e {{ v, ⌜φ v⌝}}) -∗
